extending tauto.

MirrorCharge!/src/Tauto.v
@@ -1,152 +1,288 @@
-Require Import ILogicFunc ILogic.
-Require Import MirrorCore.Ext.ExprCore.
-Require Import MirrorCore.Ext.Types.
-Require Import MirrorCore.Ext.ExprD.
-Require Import MirrorCore.Ext.ExprTactics.
 Require Import Bool.
+Require Import ExtLib.Core.RelDec.
 Require Import ExtLib.Recur.Relation.
 Require Import ExtLib.Tactics.Cases.
 Require Import ExtLib.Tactics.Injection.
+Require Import ExtLib.Tactics.EqDep.
+Require Import ExtLib.Tactics.Consider.
+Require Import Setoid Morphisms RelationClasses.
+Require Import MirrorCore.Ext.ExprCore.
+Require Import MirrorCore.Ext.Types.
+Require Import MirrorCore.EnvI.
+Require Import MirrorCore.Ext.ExprD.
+Require Import MirrorCore.Ext.ExprTactics.
+Require Import ILogicFunc ILogic.
 
-Ltac reduce_exprD := 
-	repeat match goal with
-		| H : context [ exprD _ _ _ _] |- _ => 
-		  progress (autorewrite with exprD_rw in H; simpl in H)
-	end.
-
+Set Implicit Arguments.
+Set Strict Implicit.
 
 Section Tauto.
   Context (ts : types) (funcs : fun_map ts) (gs : logic_ops ts).
-  Context (H : forall g, match gs g with
+  Context (H : forall g, match gs g return Type with
                              | Some T => @ILogic _ T
                              | None => unit
                            end).
-                           
+
   Local Instance RSym_ilfunc : SymI.RSym (typD ts) ilfunc := RSym_ilfunc ts funcs gs.
 
-Require Import ExtLib.Core.RelDec.
+  Inductive Facts : Type :=
+  | Inconsistent
+  | Knows : list (expr ilfunc) -> Facts.
 
-  Fixpoint assumption (env : list (expr ilfunc)) (p : expr ilfunc) :=
-  	match env with
-  		| nil => false
-  		| q :: env' => if p ?[eq] q then
-  					       true
-  					   else
-  					   	   assumption env' p
-  	end.
-  
-  Fixpoint tauto (env : list (expr ilfunc)) (p : expr ilfunc) : bool :=
-  match p with
-  	| Inj (ilf_true _) => true
-  	| App (App (Inj (ilf_and _)) p) q => andb (tauto env p) (tauto env q)
-  	| App (App (Inj (ilf_or _)) p) q => orb (tauto env p) (tauto env q)
-  	| App (App (Inj (ilf_impl _)) p) q => tauto (p::env) q
-  	| _ => assumption env p
-  end.
-    
-  Fixpoint eval_env (env : list (expr ilfunc)) us vs (t : typ) (ILO : ILogicOps (typD ts nil t)) 
-  	: option (typD ts nil t) :=
-  	match env with
-  		| nil => Some (@ltrue _ ILO)
-  		| p :: env => match exprD us vs p t, eval_env env us vs t ILO with
-  				 		| Some p, Some q => Some (@land _ ILO q p)
-  				 		| _, _ => None
-  				 	  end
-  	end.
+  Local Notation "P //\\ Q" := (App (App (Inj (ilf_and _)) P) Q).
 
-	Hint Extern 0 (Injective (typ_cast_typ ?A ?B ?C ?D ?E = Some ?F)) =>
-	  eapply (Injective_typ_cast_typ_hetero_Some A B C D E F) : typeclass_instances.
+  Fixpoint known_learn (e : expr ilfunc) (f : list (expr ilfunc)) : Facts :=
+    match e with
+      | Inj (ilf_true _) => Knows f
+      | Inj (ilf_false _) => Inconsistent
+      | P //\\ Q =>
+        match known_learn Q f with
+          | Inconsistent => Inconsistent
+          | Knows f => known_learn P f
+        end
+      | _ => Knows (e :: f)
+    end.
 
-Lemma assumption_sound : forall (env : list (expr ilfunc)) (p : expr ilfunc) (t : typ) us vs x v 
-    (ILO : ILogicOps (typD ts nil t))
-	(_ : exprD us vs p t = Some v) 
-	(_ : eval_env env us vs t ILO = Some x)
-    (_ : gs t = Some ILO),
-  	assumption env p = true -> @lentails (typD ts nil t) ILO x v.
-Proof.
-	intros. generalize dependent x; generalize dependent env.
-	specialize (H t); rewrite H2 in H.
-	induction env; simpl; try congruence.
-	+ intros; simpl in *.
-	Require Import ExtLib.Tactics.Consider.
-	  forward; inv_all; subst.	  
-	  consider (p ?[ eq ] a).
-	  * intros Hpa; subst. apply (@landL1 _ ILO H).
-	    rewrite H1 in H0. inv_all; subst. 
-	    Require Import Setoid Morphisms RelationClasses.
-	    admit.
-	  * intros Hpa Henv.
-	    apply (@landL1 _ ILO H).
-	    apply IHenv; auto.
-Qed.
-  
+  Definition learn e f : Facts :=
+    match f with
+      | Inconsistent => Inconsistent
+      | Knows fs => known_learn e fs
+    end.
+
+  Fixpoint known_assumption (env : list (expr ilfunc)) (p : expr ilfunc) :=
+    match env with
+      | nil => false
+      | q :: env' =>
+        if p ?[eq] q then
+  	  true
+  	else
+  	  known_assumption env' p
+    end.
+
+  Definition assumption (f : Facts) (p : expr ilfunc) : bool :=
+    match f with
+      | Inconsistent => true
+      | Knows fs => known_assumption fs p
+    end.
+
+  Fixpoint tauto (env : Facts) (p : expr ilfunc) : bool :=
+    match p with
+      | Inj (ilf_true _) => true
+      | App (App (Inj (ilf_and _)) p) q => andb (tauto env p) (tauto (learn p env) q)
+      | App (App (Inj (ilf_or _)) p) q => orb (tauto env p) (tauto env q)
+      | App (App (Inj (ilf_impl _)) p) q => tauto (learn p env) q
+      | _ => assumption env p
+    end.
+
+  Local Existing Instance lentailsPre.
+  Local Hint Extern 1 (ILogic _) => eassumption : typeclass_instances.
+
+  Section factsD.
+    Variables (us vs : env (typD ts)).
+    Variables (t : typ) (ILO : ILogicOps (typD ts nil t)).
+    Hypothesis (Hgs : gs t = Some ILO).
+
+    Fixpoint eval_env (env : list (expr ilfunc))
+    : option (typD ts nil t) :=
+      match env with
+        | nil => Some (@ltrue _ ILO)
+        | p :: env => match exprD us vs p t, eval_env env with
+  		        | Some p, Some q => Some (@land _ ILO q p)
+  		        | _, _ => None
+  		      end
+      end.
+
+    Lemma known_assumption_sound
+    : forall (env : _) (p : expr ilfunc) x v
+	     (_ : exprD us vs p t = Some v)
+	     (_ : eval_env env = Some x),
+        known_assumption env p = true ->
+        @lentails (typD ts nil t) ILO x v.
+    Proof.
+      induction env; simpl; intros; try congruence.
+      forward; inv_all; subst.
+      specialize (H t). rewrite Hgs in *.
+      consider (p ?[ eq ] a); intros; subst.
+      { rewrite H0 in *. inv_all; subst.
+        eapply landL2. reflexivity. }
+      { specialize (IHenv _ _ _ H0 eq_refl H4).
+        eapply landL1. assumption. }
+    Qed.
+
+    Definition FactsD (f : Facts) : option (typD ts nil t) :=
+      match f with
+        | Inconsistent => Some (@lfalse _ ILO)
+        | Knows fs => eval_env fs
+      end.
+
+    Lemma assumption_sound : forall (env : Facts) (p : expr ilfunc) x v
+	                            (_ : exprD us vs p t = Some v)
+	                            (_ : FactsD env = Some x)
+                                    (_ : gs t = Some ILO),
+                               assumption env p = true ->
+                               @lentails (typD ts nil t) ILO x v.
+    Proof.
+      destruct env; simpl; intros; inv_all; subst.
+      { specialize (H t). rewrite H2 in *.
+        eapply lfalseL. }
+      { eapply known_assumption_sound; eauto. }
+    Qed.
+
+    Lemma FactsD_known_cons
+    : forall (f : list (expr ilfunc))
+             (v : typD ts nil t)
+             (P : typD ts nil t)
+             (e : expr ilfunc),
+        eval_env f = Some P ->
+        exprD us vs e t = Some v ->
+        exists Q : typD ts nil t,
+          FactsD (Knows (e :: f)) = Some Q /\ land P v |-- Q.
+    Proof.
+      admit.
+    Qed.
+
+    Lemma FactsD_known_learn : forall e f f' v P,
+      exprD us vs e t = Some v ->
+      eval_env f = Some P ->
+      known_learn e f = f' ->
+      exists Q,
+        FactsD f' = Some Q /\
+        land P v |-- Q.
+    Proof.
+      refine (@expr_strong_ind _ _ _); intros.
+      destruct e; subst; eauto using FactsD_known_cons.
+      { simpl. destruct i; eauto using FactsD_known_cons.
+        { red_exprD. simpl in *.
+          forward; inv_all; subst.
+          rewrite H2. eexists; split; eauto.
+          specialize (H t). 
+          rewrite H1 in *. inv_all; subst.
+          apply landL1. reflexivity. }
+        { red_exprD; simpl in *.
+          forward; inv_all; subst.
+          eexists; split; eauto.
+          specialize (H t). rewrite H1 in *. inv_all; subst.
+          eapply landL2. reflexivity. } }
+      { simpl.
+        destruct e1; eauto using FactsD_known_cons.
+        destruct e1_1; eauto using FactsD_known_cons.
+        destruct i; eauto using FactsD_known_cons.
+        repeat (red_exprD; Cases.rewrite_all; forward; simpl in *; inv_all; try subst).
+        revert H11. repeat subst.
+        rewrite typ_cast_typ_refl in *. inv_all; subst.
+        intros; subst. specialize (H t). rewrite H3 in *. inv_all; subst.
+        consider (known_learn e2 f); intros.
+        { eexists; split. reflexivity.
+          eapply H0 in H1; eauto with typeclass_instances.
+          destruct H1. destruct H1.
+          simpl in H1. inv_all. subst.
+          etransitivity. 2: eassumption.
+          eapply landR.
+          { eapply landL1. reflexivity. }
+          { eapply landL2. eapply landL2. reflexivity. } }
+        { eapply H0 in H1; eauto with typeclass_instances.
+          destruct H1. destruct H1. simpl in H1.
+          consider (known_learn e1_2 l); simpl; intros.
+          { eexists; split; eauto.
+            eapply H0 in H6; try eassumption; eauto with typeclass_instances.
+            destruct H6. destruct H6.
+            simpl in *. inv_all; subst.
+            etransitivity; [ | eassumption ].
+            eapply landR.
+            { etransitivity; [ | eassumption ].
+              eapply landR.
+              { eapply landL1. reflexivity. }
+              { eapply landL2; eapply landL2; reflexivity. } }
+            { eapply landL2. eapply landL1. reflexivity. } }
+          { eapply H0 in H6. 4: eassumption. 2: eauto with typeclass_instances.
+            2: eauto.
+            destruct H6. destruct H6.
+            eexists; split; eauto.
+            etransitivity; [ | eassumption ].
+            eapply landR.
+            { etransitivity; [ | eassumption ].
+              eapply landR.
+              { eapply landL1. reflexivity. }
+              { eapply landL2. eapply landL2. reflexivity. } }
+            { eapply landL2. eapply landL1. reflexivity. } } } }
+    Qed.
+
+    Lemma FactsD_learn : forall f f' e v P,
+      exprD us vs e t = Some v ->
+      FactsD f = Some P ->
+      learn e f = f' ->
+      exists Q,
+        FactsD f' = Some Q /\
+        land P v |-- Q.
+    Proof.
+      destruct f; simpl; intros; inv_all; subst.
+      { exists lfalse. intuition.
+        specialize (H t). rewrite Hgs in *.
+        eapply landL1. reflexivity. }
+      { eapply FactsD_known_learn; eauto. }
+    Qed.
+
+  End factsD.
+
   Lemma tauto_sound : forall (p : expr ilfunc) (t : typ) env us vs x v
-    (_ : exprD us vs p t = Some v) 
+    (_ : exprD us vs p t = Some v)
     (ILO : ILogicOps (typD ts nil t))
     (_ : gs t = Some ILO)
- 	(_ : eval_env env us vs t ILO = Some x),
-  	tauto env p = true -> @lentails (typD ts nil t) ILO x v.
+    (_ : FactsD us vs t ILO env = Some x),
+    tauto env p = true ->
+    @lentails (typD ts nil t) ILO x v.
   Proof.
-    intro p.
-    apply expr_strong_ind with (e := p); clear p; intros.
-    destruct e; simpl in *; try (eauto using assumption_sound).
-    
-    destruct i; eauto using assumption_sound.
-	reduce_exprD;  unfold SymI.symAs in H1. simpl in H1.
-	forward. inv_all. destruct H5; subst.
-	specialize (H t); rewrite H1 in *. inv_all; subst. 
-	apply (@ltrueR _ ILO H).
-
-    destruct e1; eauto using assumption_sound.
-    destruct e1_1; eauto using assumption_sound.
-    destruct i; eauto using assumption_sound.
-	+ repeat progress (reduce_exprD; forward; inv_all; try subst).
-	  revert H14; subst.
-	  unfold SymI.symAs in H9; simpl in H9. forward. inv_all; subst. 
-
-	  repeat (match goal with
-	  		   | H : exists x, _ |- _ => destruct H; intuition; subst
-	  		  end). inv_all; subst.
-	  		  inversion x1; subst. subst.
-	  		  	  		  Require Import ExtLib.Tactics.EqDep.
-	  		  
-	  		  uip_all.
-	rewrite Bool.andb_true_iff in H4. destruct H4 as [H4 H5].
-	rewrite H1 in H2. inversion H2; subst.
-	specialize (H t). rewrite H1 in H.
-	apply (@landR _ _ H); eapply H0; try eassumption; red; solve_expr_acc_trans.
-
-	+ repeat progress (reduce_exprD; forward; inv_all; try subst).
-	  revert H14; repeat subst. intros.
-	  unfold SymI.symAs in H9; simpl in H9; forward; inv_all; subst.
-	  repeat (match goal with
-	  		   | H : exists x, _ |- _ => destruct H; intuition; subst
-	  		  end). inv_all; subst.
-	  		  inversion x1; subst. subst.
-	  		  	  		  Require Import ExtLib.Tactics.EqDep.
-	  		  
-	  		  uip_all.
-	rewrite H2 in *; inv_all; subst.
-	specialize (H t). rewrite H2 in H.
-	rewrite Bool.orb_true_iff in H4. destruct H4 as [H4 | H4].
-	apply (@lorR1 _ i H); eapply H0; try eassumption; red; solve_expr_acc_trans.
-	apply (@lorR2 _ i H); eapply H0; try eassumption; red; solve_expr_acc_trans.
-	+ repeat progress (reduce_exprD; forward; inv_all; try subst).
-	  revert H14; subst; intros.
-	  unfold SymI.symAs in H9; simpl in H9; forward; inv_all; subst.
-	  repeat (match goal with
-	  		   | H : exists x, _ |- _ => destruct H; intuition; subst
-	  		  end). inv_all; subst.
-	  		  inversion x1; subst. subst.
-	  		  uip_all.
-	  		  simpl in *.
-	rewrite H1 in H2. inversion H2; subst.
-	specialize (H t). rewrite H1 in H.
-	  
-	apply (@limplAdj _ _ H).
-	eapply H0; try eassumption.
-	* red; solve_expr_acc_trans.
-	* simpl. rewrite H12, H3. reflexivity.
-Qed.	
+    refine (@expr_strong_ind _ _ _); intros.
+    destruct e; simpl in *; eauto using assumption_sound.
+    { destruct i; eauto using assumption_sound.
+      red_exprD. simpl in *.
+      forward; inv_all; subst.
+      specialize (H t).
+      rewrite H1 in *. inv_all; subst.
+      eapply ltrueR. }
+    { destruct e1; eauto using assumption_sound.
+      destruct e1_1; eauto using assumption_sound.
+      destruct i; eauto using assumption_sound.
+      { eapply andb_true_iff in H4. destruct H4.
+        repeat (red_exprD; forward; inv_all; subst).
+        red_exprD. rewrite H6 in *.
+        red_exprD. rewrite H6 in *.
+        rewrite typ_cast_typ_refl in *.
+        simpl in *. forward; subst. inv_all; subst.
+        inversion x0; subst. clear H9.
+        uip_all'.
+        rewrite H6 in H2. inv_all; subst.
+        specialize (H t). rewrite H6 in *.
+        eapply landR.
+        { eapply H0; eauto.
+          eauto with typeclass_instances. }
+        { destruct (@FactsD_learn us vs _ _ H6 env (learn e1_2 env) e1_2 t1 x H7 H3 eq_refl).
+          destruct H1.
+          eapply H0 in H5. 5: eassumption. 4: eauto. 3: eauto. 2: eauto with typeclass_instances.
+          etransitivity; [ | eassumption ].
+          etransitivity; [ | eassumption ].
+          eapply landR; eauto.
+          { eapply H0; eauto. eauto with typeclass_instances. } } }
+      { eapply orb_true_iff in H4.
+        repeat (red_exprD; forward; inv_all; simpl in *; try subst).
+        revert H13. repeat subst.
+        specialize (H t).
+        rewrite H5 in *. inv_all; subst.
+        uip_all'; intros. subst.
+        destruct H4.
+        { eapply lorR1. eapply H0; eauto. eauto with typeclass_instances. }
+        { eapply lorR2. eapply H0; eauto. eauto with typeclass_instances. } }
+      { repeat (red_exprD; forward; inv_all; simpl in *; try subst).
+        revert H13; repeat subst.
+        uip_all'. intros; subst.
+        specialize (H t).
+        rewrite H5 in *; inv_all; subst.
+        eapply limplAdj.
+        destruct (@FactsD_learn us vs _ _ H5 env _ _ _ _ H9 H3 eq_refl).
+        destruct H2.
+        etransitivity.
+        2: eapply H0. 6: eassumption. 5: eassumption. 4: eauto. 3: eauto. 2: eauto with typeclass_instances.
+        eauto. } }
+  Qed.
 
 End Tauto.
